examples/hoare_logic/blocking_semantics3/blocking_semantics3_ImpExpr_steps_non_neg_2.v
@@ -96,11 +96,6 @@ Existing Instance term_WhyType.
 Axiom term_node_WhyType : WhyType term_node.
 Existing Instance term_node_WhyType.
 
-Scheme term_induc := Induction for term Sort Prop 
-   with term_node_induc := Induction for term_node Sort Prop.
-
-Print term_induc.
-
 (* Why3 assumption *)
 Definition term_maxvar(v:term): Z := match v with
   | (mk_term x x1) => x1
@@ -158,8 +153,6 @@ Inductive fmla  :=
   | Fforall : ident -> datatype -> fmla -> fmla .
 Axiom fmla_WhyType : WhyType fmla.
 Existing Instance fmla_WhyType.
-
-Print fmla_ind.
 
 (* Why3 assumption *)
 Inductive stmt  :=
@@ -376,58 +369,167 @@ Axiom fresh_in_binop : forall (t:term) (t':term) (op:operator) (v:ident),
   (fresh_in_term v (mk_tbin t op t')) -> ((fresh_in_term v t) /\
   (fresh_in_term v t')).
 
-Require Import Why3.
+Axiom eval_msubst_term : forall (e:term) (sigma:(map mident value)) (pi:(list
+  (ident* value)%type)) (x:mident) (v:ident), (fresh_in_term v e) ->
+  ((eval_term sigma pi (msubst_term e x v)) = (eval_term (set sigma x
+  (get_stack v pi)) pi e)).
 
-Ltac ae := why3 "alt-ergo" timelimit 3.
+Axiom eval_subst_term : forall (sigma:(map mident value)) (pi:(list (ident*
+  value)%type)) (e:term) (x:ident) (v:ident), (fresh_in_term v e) ->
+  ((eval_term sigma pi (subst_term e x v)) = (eval_term sigma (Cons (x,
+  (get_stack v pi)) pi) e)).
+
+Axiom eval_term_change_free : forall (t:term) (sigma:(map mident value))
+  (pi:(list (ident* value)%type)) (id:ident) (v:value), (fresh_in_term id
+  t) -> ((eval_term sigma (Cons (id, v) pi) t) = (eval_term sigma pi t)).
+
+(* Why3 assumption *)
+Fixpoint fresh_in_fmla(id:ident) (f:fmla) {struct f}: Prop :=
+  match f with
+  | (Fterm e) => (fresh_in_term id e)
+  | ((Fand f1 f2)|(Fimplies f1 f2)) => (fresh_in_fmla id f1) /\
+      (fresh_in_fmla id f2)
+  | (Fnot f1) => (fresh_in_fmla id f1)
+  | (Flet y t f1) => (~ (id = y)) /\ ((fresh_in_term id t) /\
+      (fresh_in_fmla id f1))
+  | (Fforall y ty f1) => (~ (id = y)) /\ (fresh_in_fmla id f1)
+  end.
+
+(* Why3 assumption *)
+Fixpoint subst(f:fmla) (x:ident) (v:ident) {struct f}: fmla :=
+  match f with
+  | (Fterm e) => (Fterm (subst_term e x v))
+  | (Fand f1 f2) => (Fand (subst f1 x v) (subst f2 x v))
+  | (Fnot f1) => (Fnot (subst f1 x v))
+  | (Fimplies f1 f2) => (Fimplies (subst f1 x v) (subst f2 x v))
+  | (Flet y t f1) => (Flet y (subst_term t x v) (subst f1 x v))
+  | (Fforall y ty f1) => (Fforall y ty (subst f1 x v))
+  end.
+
+(* Why3 assumption *)
+Fixpoint msubst(f:fmla) (x:mident) (v:ident) {struct f}: fmla :=
+  match f with
+  | (Fterm e) => (Fterm (msubst_term e x v))
+  | (Fand f1 f2) => (Fand (msubst f1 x v) (msubst f2 x v))
+  | (Fnot f1) => (Fnot (msubst f1 x v))
+  | (Fimplies f1 f2) => (Fimplies (msubst f1 x v) (msubst f2 x v))
+  | (Flet y t f1) => (Flet y (msubst_term t x v) (msubst f1 x v))
+  | (Fforall y ty f1) => (Fforall y ty (msubst f1 x v))
+  end.
+
+Axiom subst_fresh : forall (f:fmla) (x:ident) (v:ident), (fresh_in_fmla x
+  f) -> ((subst f x v) = f).
+
+Axiom let_subst : forall (t:term) (f:fmla) (x:ident) (id':ident) (id:mident),
+  ((msubst (Flet x t f) id id') = (Flet x (msubst_term t id id') (msubst f id
+  id'))).
+
+Axiom eval_msubst : forall (f:fmla) (sigma:(map mident value)) (pi:(list
+  (ident* value)%type)) (x:mident) (v:ident), (fresh_in_fmla v f) ->
+  ((eval_fmla sigma pi (msubst f x v)) <-> (eval_fmla (set sigma x
+  (get_stack v pi)) pi f)).
+
+Axiom eval_subst : forall (f:fmla) (sigma:(map mident value)) (pi:(list
+  (ident* value)%type)) (x:ident) (v:ident), (fresh_in_fmla v f) ->
+  ((eval_fmla sigma pi (subst f x v)) <-> (eval_fmla sigma (Cons (x,
+  (get_stack v pi)) pi) f)).
+
+Axiom eval_swap : forall (f:fmla) (sigma:(map mident value)) (pi:(list
+  (ident* value)%type)) (id1:ident) (id2:ident) (v1:value) (v2:value),
+  (~ (id1 = id2)) -> ((eval_fmla sigma (Cons (id1, v1) (Cons (id2, v2) pi))
+  f) <-> (eval_fmla sigma (Cons (id2, v2) (Cons (id1, v1) pi)) f)).
+
+Axiom eval_same_var : forall (f:fmla) (sigma:(map mident value)) (pi:(list
+  (ident* value)%type)) (id:ident) (v1:value) (v2:value), (eval_fmla sigma
+  (Cons (id, v1) (Cons (id, v2) pi)) f) <-> (eval_fmla sigma (Cons (id, v1)
+  pi) f).
+
+Axiom eval_change_free : forall (f:fmla) (sigma:(map mident value)) (pi:(list
+  (ident* value)%type)) (id:ident) (v:value), (fresh_in_fmla id f) ->
+  ((eval_fmla sigma (Cons (id, v) pi) f) <-> (eval_fmla sigma pi f)).
+
+(* Why3 assumption *)
+Definition valid_fmla(p:fmla): Prop := forall (sigma:(map mident value))
+  (pi:(list (ident* value)%type)), (eval_fmla sigma pi p).
+
+Axiom msubst_implies : forall (p:fmla) (q:fmla), (valid_fmla (Fimplies p
+  q)) -> forall (sigma:(map mident value)) (pi:(list (ident* value)%type))
+  (x:mident) (id:ident), (fresh_in_fmla id (Fand p q)) -> (eval_fmla sigma
+  (Cons (id, (get sigma x)) pi) (Fimplies (msubst p x id) (msubst q x id))).
+
+Axiom let_equiv : forall (id:ident) (id':ident) (t:term) (f:fmla),
+  forall (sigma:(map mident value)) (pi:(list (ident* value)%type)),
+  (fresh_in_fmla id' f) -> ((eval_fmla sigma pi (Flet id' t (subst f id
+  id'))) -> (eval_fmla sigma pi (Flet id t f))).
+
+Axiom let_implies : forall (id:ident) (t:term) (p:fmla) (q:fmla),
+  (valid_fmla (Fimplies p q)) -> (valid_fmla (Fimplies (Flet id t p) (Flet id
+  t q))).
+
+(* Why3 assumption *)
+Fixpoint fresh_in_stmt(id:ident) (s:stmt) {struct s}: Prop :=
+  match s with
+  | Sskip => True
+  | (Sseq s1 s2) => (fresh_in_stmt id s1) /\ (fresh_in_stmt id s2)
+  | (Sassign _ t) => (fresh_in_term id t)
+  | (Sif t s1 s2) => (fresh_in_term id t) /\ ((fresh_in_stmt id s1) /\
+      (fresh_in_stmt id s2))
+  | (Sassert f) => (fresh_in_fmla id f)
+  | (Swhile cond inv body) => (fresh_in_term id cond) /\ ((fresh_in_fmla id
+      inv) /\ (fresh_in_stmt id body))
+  end.
+
+(* Why3 assumption *)
+Inductive one_step : (map mident value) -> (list (ident* value)%type) -> stmt
+  -> (map mident value) -> (list (ident* value)%type) -> stmt -> Prop :=
+  | one_step_assign : forall (sigma:(map mident value)) (sigma':(map mident
+      value)) (pi:(list (ident* value)%type)) (x:mident) (t:term),
+      (sigma' = (set sigma x (eval_term sigma pi t))) -> (one_step sigma pi
+      (Sassign x t) sigma' pi Sskip)
+  | one_step_seq_noskip : forall (sigma:(map mident value)) (sigma':(map
+      mident value)) (pi:(list (ident* value)%type)) (pi':(list (ident*
+      value)%type)) (s1:stmt) (s1':stmt) (s2:stmt), (one_step sigma pi s1
+      sigma' pi' s1') -> (one_step sigma pi (Sseq s1 s2) sigma' pi' (Sseq s1'
+      s2))
+  | one_step_seq_skip : forall (sigma:(map mident value)) (pi:(list (ident*
+      value)%type)) (s:stmt), (one_step sigma pi (Sseq Sskip s) sigma pi s)
+  | one_step_if_true : forall (sigma:(map mident value)) (pi:(list (ident*
+      value)%type)) (t:term) (s1:stmt) (s2:stmt), ((eval_term sigma pi
+      t) = (Vbool true)) -> (one_step sigma pi (Sif t s1 s2) sigma pi s1)
+  | one_step_if_false : forall (sigma:(map mident value)) (pi:(list (ident*
+      value)%type)) (t:term) (s1:stmt) (s2:stmt), ((eval_term sigma pi
+      t) = (Vbool false)) -> (one_step sigma pi (Sif t s1 s2) sigma pi s2)
+  | one_step_assert : forall (sigma:(map mident value)) (pi:(list (ident*
+      value)%type)) (f:fmla), (eval_fmla sigma pi f) -> (one_step sigma pi
+      (Sassert f) sigma pi Sskip)
+  | one_step_while_true : forall (sigma:(map mident value)) (pi:(list (ident*
+      value)%type)) (cond:term) (inv:fmla) (body:stmt), (eval_fmla sigma pi
+      inv) -> (((eval_term sigma pi cond) = (Vbool true)) -> (one_step sigma
+      pi (Swhile cond inv body) sigma pi (Sseq body (Swhile cond inv body))))
+  | one_step_while_false : forall (sigma:(map mident value)) (pi:(list
+      (ident* value)%type)) (cond:term) (inv:fmla) (body:stmt),
+      (eval_fmla sigma pi inv) -> (((eval_term sigma pi
+      cond) = (Vbool false)) -> (one_step sigma pi (Swhile cond inv body)
+      sigma pi Sskip)).
+
+(* Why3 assumption *)
+Inductive many_steps : (map mident value) -> (list (ident* value)%type)
+  -> stmt -> (map mident value) -> (list (ident* value)%type) -> stmt
+  -> Z -> Prop :=
+  | many_steps_refl : forall (sigma:(map mident value)) (pi:(list (ident*
+      value)%type)) (s:stmt), (many_steps sigma pi s sigma pi s 0%Z)
+  | many_steps_trans : forall (sigma1:(map mident value)) (sigma2:(map mident
+      value)) (sigma3:(map mident value)) (pi1:(list (ident* value)%type))
+      (pi2:(list (ident* value)%type)) (pi3:(list (ident* value)%type))
+      (s1:stmt) (s2:stmt) (s3:stmt) (n:Z), (one_step sigma1 pi1 s1 sigma2 pi2
+      s2) -> ((many_steps sigma2 pi2 s2 sigma3 pi3 s3 n) ->
+      (many_steps sigma1 pi1 s1 sigma3 pi3 s3 (n + 1%Z)%Z)).
 
 (* Why3 goal *)
-Theorem eval_msubst_term : forall (e:term) (sigma:(map mident value))
-  (pi:(list (ident* value)%type)) (x:mident) (v:ident), (fresh_in_term v
-  e) -> ((eval_term sigma pi (msubst_term e x v)) = (eval_term (set sigma x
-  (get_stack v pi)) pi e)).
-Check term_induc.
-intros e.
-apply term_induc with (P := fun e => 
-  forall (sigma : map mident value) (pi : list (ident * value))
-     (x : mident) (v : ident),
-     fresh_in_term v e ->
-     eval_term sigma pi (msubst_term e x v) =
-     eval_term (set sigma x (get_stack v pi)) pi e) 
-     (P0 := fun t => 
-       forall (i : int) (sigma : map mident value) (pi : list (ident * value))
-       (x : mident) (v : ident),
-       fresh_in_term v (mk_term t i) ->
-       eval_term sigma pi (msubst_term (mk_term t i) x v) =
-       eval_term (set sigma x (get_stack v pi)) pi (mk_term t i)).
-(* mk_term*)
-ae.
-(* Value *)
-ae.
-(* Var *)
-intros i i0 sigma pi x v H.
-simpl.
-rewrite (msubst_term_def (mk_term (Tvar i) i0)).
-easy.
-(* Ref *)
-intros m i sigma pi x v H.
-simpl.
-destruct (mident_decide m x).
-(* m = x*)
-ae.
-(* m <> x*)
-ae.
-(* Bin *)
-intros t H1.
-intros op t' H2.
-intros i sigma pi x v H3.
-rewrite (msubst_term_def (mk_term (Tbin t op t') i)).
-simpl.
-rewrite H1.
-rewrite H2; auto.
-apply fresh_in_binop with (t:=t) (t':=t') (op := op).
-apply fresh_in_binop with (t:=t) (t':=t') (op := op);
-admit.
-
+Theorem steps_non_neg : forall (sigma1:(map mident value)) (sigma2:(map
+  mident value)) (pi1:(list (ident* value)%type)) (pi2:(list (ident*
+  value)%type)) (s1:stmt) (s2:stmt) (n:Z), (many_steps sigma1 pi1 s1 sigma2
+  pi2 s2 n) -> (0%Z <= n)%Z.
+intros sigma1 sigma2 pi1 pi2 s1 s2 n.
+induction 1; omega.
 Qed.
-
-
